

Backup

$$
\begin{align}
\mathbb{V}\left(
\hat{\tau}^{\text{dm}}
\right)
&=
\mathbb{V}\left(
\frac{1}{n_t}\sum_{W_i=1}Y_i - \frac{1}{n_c}\sum_{W_i=0}Y_i
\right)
\\[5pt]
&\text{\href{#lemma-1}{Lemma 1}}
\\[5pt]
&=
\mathbb{V}\left(
\frac{1}{n_t}\sum_{i=1}^n W_iY_i - \frac{1}{n_c}\sum_{i=1}^n (1-W_i)Y_i
\right)
\\[5pt]
&\text{\href{#lemma-2}{Lemma 2}}
\\[5pt]
&=
\mathbb{V}\left(
\frac{1}{n_t}\sum_{i=1}^n W_iY_i(1) - \frac{1}{n_c}\sum_{i=1}^n (1-W_i)Y_i(0)
\right)
\\[5pt]
&=
\mathbb{V}\left(
\frac{1}{n_t}\sum_{i=1}^n W_iY_i(1) 
- \frac{1}{n_c}\sum_{i=1}^n Y_i(0)
+ \frac{1}{n_c}\sum_{i=1}^n W_iY_i(0)
\right)
\\[5pt]
&=
\mathbb{V}\left(
\sum_{i=1}^n W_i\frac{Y_i(1)}{n_t} 
- \sum_{i=1}^n \frac{Y_i(0)}{n_c}
+ \sum_{i=1}^n W_i\frac{Y_i(0)}{n_c}
\right)
\\[5pt]
&=
\mathbb{V}\left(
\sum_{i=1}^n W_i \left(\frac{Y_i(1)}{n_t} + \frac{Y_i(0)}{n_c}\right)
- \sum_{i=1}^n \frac{Y_i(0)}{n_c}
\right)
\\[5pt]
&\text{Drop constant (variance unchanged)}
\\[5pt]
&=
\mathbb{V}\left(
\sum_{i=1}^n W_i \left(\frac{Y_i(1)}{n_t} + \frac{Y_i(0)}{n_c}\right)
\right)
\\[5pt]
&\text{Demean (variance unchanged)}
\\[5pt]
&= 
\mathbb{V}\left(\sum_{i=1}^n W_i \left(\frac{Y_i(1)}{n_t} + \frac{Y_i(0)}{n_c} - \left(\frac{\overline{Y}(1)}{n_t} + \frac{\overline{Y}(0)}{n_c}\right)
\right)\right)
&\text{}
\\[5pt]
&\text{Using shorthands } Y_i^+ \coloneqq Y_i(1)/n_t + Y_i(0)/n_c \text{ and } \overline{Y}^+ \coloneqq \overline{Y}(1)/n_t + \overline{Y}(0)/n_c
\\[5pt]
&= 
\mathbb{V}\left(\sum_{i=1}^n W_i \left(Y_i^+ - \overline{Y}^+
\right)\right)
&\text{}
\\[5pt]
&\text{Rewriting variance in terms of covariance}
\\[5pt]
&= 
\text{Cov}\left(
\sum_{i=1}^n W_i \left(Y_i^+ - \overline{Y}^+\right),
\sum_{j=1}^n W_j \left(Y_j^+ - \overline{Y}^+\right)
\right)
&\text{}
\\[5pt]
&= 
\sum_{i=1}^n \sum_{j=1}^n
\text{Cov}\left(
W_i \left(Y_i^+ - \overline{Y}^+\right),
W_j \left(Y_j^+ - \overline{Y}^+\right)
\right)
&\text{}
\\[5pt]
&= 
\sum_{i=1}^n \sum_{j=1}^n
\text{Cov}\left(W_i, W_j \right)
\left(Y_i^+ - \overline{Y}^+\right)
\left(Y_j^+ - \overline{Y}^+\right)
&\text{}
\\[5pt]
&= 
\sum_{i=1}^n
\mathbb{V}\left(W_i^2\right)
\left(Y_i^+ - \overline{Y}^+\right)^2
+
\sum_{i=1}^n \sum_{j \neq i}
\text{Cov}\left(W_i, W_j \right)
\left(Y_i^+ - \overline{Y}^+\right)
\left(Y_j^+ - \overline{Y}^+\right)
&\text{}
\\[5pt]
&\text{Lemma 2}
\\[5pt]
&= 
\sum_{i=1}^n
\mathbb{V}\left(W_i\right)
\left(Y_i^+ - \overline{Y}^+\right)^2
+
\sum_{i=1}^n \sum_{j \neq i}
\text{Cov}\left(W_i, W_j \right)
\left(Y_i^+ - \overline{Y}^+\right)
\left(Y_j^+ - \overline{Y}^+\right)
&\text{}
\\[5pt]
&\text{Lemma 3}
\\[5pt]
&=
\sum_{i=1}^{n}\left(\frac{n_tn_c}{n^2}\right)
\left(Y_i^+ - \overline{Y}^+\right)^2
- \sum_{i=1}^{n}\sum_{j \neq i}\left(\frac{n_tn_c}{n^2(n-1)}\right)
\left(Y_i^+ - \overline{Y}^+\right)\left(Y_j^+ - \overline{Y}^+\right)
\\[5pt]
&=
\left(\frac{n_tn_c}{n^2}\right)
\sum_{i=1}^{n}\left(Y_i^+ - \overline{Y}^+\right)^2
- \left(\frac{n_tn_c}{n^2(n-1)}\right)\sum_{i=1}^{n}\sum_{j \neq i}
\left(Y_i^+ - \overline{Y}^+\right)\left(Y_j^+ - \overline{Y}^+\right)
\\[5pt]
&\text{Lemma 4}
\\[5pt]
&=
\left(\frac{n_tn_c}{n^2}\right)
\sum_{i=1}^{n}\left(Y_i^+ - \overline{Y}^+\right)^2
+ \left(\frac{n_tn_c}{n^2(n-1)}\right)\sum_{i=1}^{n}
\left(Y_i^+ - \overline{Y}^+\right)^2
\\[5pt]
&=
\left(\frac{n_tn_c}{n^2} + \frac{n_tn_c}{n^2(n-1)}\right)
\sum_{i=1}^{n}\left(Y_i^+ - \overline{Y}^+\right)^2
&\\[5pt]
&=
\frac{n_tn_c(n-1) + n_tn_c}{n^2(n-1)}
\sum_{i=1}^{n}\left(Y_i^+ - \overline{Y}^+\right)^2
&\\[5pt]
&=
\frac{nn_tn_c - n_tn_c + n_tn_c}{n^2(n-1)}
\sum_{i=1}^{n}\left(Y_i^+ - \overline{Y}^+\right)^2
&\\[5pt]
&=
\frac{n_tn_c}{n(n-1)}
\sum_{i=1}^{n}\left(Y_i^+ - \overline{Y}^+\right)^2
&\\[5pt]
&\text{Reverting to full notation and expanding square term}
\\[5pt]
&=
\frac{n_tn_c}{n(n-1)}
\sum_{i=1}^{n}\left(\frac{Y_i(1)}{n_t} + \frac{Y_i(0)}{n_c} - \left(\frac{\overline{Y}(1)}{n_t} + \frac{\overline{Y}(0)}{n_c}\right)\right)^2
&\text{}
\\[5pt]
&=
\frac{n_tn_c}{n(n-1)}
\sum_{i=1}^{n}\left(\frac{Y_i(1)}{n_t} + \frac{Y_i(0)}{n_c} 
- \frac{\overline{Y}(1)}{n_t} - \frac{\overline{Y}(0)}{n_c}\right)^2
&\text{}
\\[5pt]
&=
\frac{n_tn_c}{n(n-1)}
\sum_{i=1}^{n}\left(
\left(\frac{Y_i(1)}{n_t} - \frac{\overline{Y}(1)}{n_t}\right)
+ \left(\frac{Y_i(0)}{n_c} - \frac{\overline{Y}(0)}{n_c}\right)
\right)^2
&\text{}
\\[5pt]
&=
\frac{n_tn_c}{n(n-1)}
\sum_{i=1}^{n}\left(
\frac{1}{n_t}\left(Y_i(1) - \overline{Y}(1)\right)
+ \frac{1}{n_c}\left(Y_i(0) - \overline{Y}(0)\right)
\right)^2
&\text{}
\\[5pt]
&=
\frac{n_tn_c}{n(n-1)}\left[
\sum_{i=1}^{n}\left(
\frac{1}{n_t^2}\left(Y_i(1) - \overline{Y}(1)\right)^2
+ \frac{1}{n_c^2}\left(Y_i(0) - \overline{Y}(0)\right)^2
+ \frac{2}{n_t n_c}\left(Y_i(1) - \overline{Y}(1)\right)\left(Y_i(0) - \overline{Y}(0)\right)
\right)
\right]
&\text{}
\\[5pt]
&=
\frac{n_tn_c}{n(n-1)}\left[
\frac{1}{n_t^2}\sum_{i=1}^{n}\left(Y_i(1) - \overline{Y}(1)\right)^2
+ \frac{1}{n_c^2}\sum_{i=1}^{n}\left(Y_i(0) - \overline{Y}(0)\right)^2
+ \frac{2}{n_t n_c}\sum_{i=1}^{n}\left(Y_i(1) - \overline{Y}(1)\right)\left(Y_i(0) - \overline{Y}(0)\right)
\right]
&\text{}
\\[5pt]
&=
\frac{n_c}{n n_t}\frac{1}{n-1}\sum_{i=1}^{n}\left(Y_i(1) - \overline{Y}(1)\right)^2
+ \frac{n_t}{n n_c}\frac{1}{n-1}\sum_{i=1}^{n}\left(Y_i(0) - \overline{Y}(0)\right)^2
+ \frac{2}{n}\frac{1}{n-1}\sum_{i=1}^{n}\left(Y_i(1) - \overline{Y}(1)\right)\left(Y_i(0) - \overline{Y}(0)\right)
&\text{}
\\[5pt]
&=
\frac{n_c}{n n_t}S_1^2
+ \frac{n_t}{n n_c}S_0^2
+ \frac{1}{n}2S_{0,1}
&\text{}
\\[5pt]
&\text{Lemma 5}
\\[5pt]
&=
\frac{n_c}{n n_t}S_1^2
+ \frac{n_t}{n n_c}S_0^2
+ \frac{1}{n}\left(S_1^2 + S_0^2 - S_{\tau_i}^2\right)
&\text{}
\\[5pt]
&=
\left(\frac{n_c}{n n_t} + \frac{1}{n}\right)S_1^2
+ \left(\frac{n_t}{n n_c} + \frac{1}{n}\right) S_0^2
- \frac{S_{\tau_i}^2}{n}
&\text{}
\\[5pt]
&=
\frac{n_c + n_t}{n n_t} S_1^2
+ \frac{n_t + n_c}{n n_c} S_0^2
- \frac{S_{\tau_i}^2}{n}
&\text{}
\\[5pt]
&=
\frac{S_1^2}{n_t}
+ \frac{S_0^2}{n_c} 
- \frac{S_{\tau_i}^2}{n}
&\text{}
\\[5pt]
\end{align}
$${#eq-var}






This is the [sampling variance](stats_foundations.md#sampling-distribution) of $\hat{\tau}^{\text{dm}}$. It's a theoretical quantity we cannot directly observe. 




## Lemmas
### Lemma 1 {#lemma-1}
Given that $W_i=1$ for treatment units and $W_i=0$ for control units, we can calculate treatment group means by summing over all units and using $W_i$ to "pick out" the relevant units for each treatment group so that we have:
$$
\begin{align}
\hat{\tau}^{\text{dm}}
&=
\frac{1}{n_t}\sum_{W_i=1}Y_i - \frac{1}{n_c}\sum_{W_i=0}Y_i
\\[5pt]
&= 
\frac{1}{n_t}\sum_{i=1}^{n}W_iY_i - \frac{1}{n_c}\sum_{i=1}^{n}(1-W_i)Y_i
\end{align}
$$
[↩️](#main-derivation)

### Lemma 2 {#lemma-2} 
This step uses [SUTVA](unbiasedness.md#sutva-links-observed-outcomes-to-potential-outcomes) which – if it holds – implies that:
$$
Y_i = Y_i(W_i) = \begin{cases} 
   Y_i(1) & \text{if } W_i = 1 \\
   Y_i(0)       & \text{if } W_i = 0,
  \end{cases}
$$[↩️](#main-derivation)

### Lemma 3 {#lemma-3}
Here we're using the facts that:
$$
\begin{align}
\mathbb{V}\Bigl(\sum_i X_ia\Bigr)
&= \text{Cov}\Bigl(\sum_i X_ia, \sum_j X_ja\Bigr) \\[6pt]
&= \sum_i\sum_j\text{Cov}\Bigl( X_ia,  X_ja\Bigr) \\[6pt]
&= \sum_i \sum_j \text{Cov}(X_i, X_j) aa \\[6pt]
\end{align}
$$
[↩️](#main-derivation)
